synth_bitfield_recip_inverse

src/lowparse/LowParse.Spec.BitFields.fst
@@ -23,98 +23,136 @@ let rec bounds_of_widths (lo: nat) (hi: nat { lo <= hi }) (l: list nat) : Pure (
   | [_] -> []
   | sz :: q -> (lo + sz) :: bounds_of_widths (lo + sz) hi q
 
-let rec bitfields (tot: pos) (lo: nat) (hi: nat { lo <= hi /\ hi <= tot }) (l: list nat { valid_bitfield_widths lo hi l }) : Tot Type0 (decreases l) =
-  match l with
-  | [] -> unit
-  | [sz] -> BF.bitfield tot sz
-  | sz :: q -> BF.bitfield tot sz & bitfields tot (lo + sz) hi q
-
 module U = FStar.UInt
 
-let rec synth_bitfield (tot: pos) (lo: nat) (hi: nat { lo <= hi /\ hi <= tot }) (l: list nat { valid_bitfield_widths lo hi l }) (x: U.uint_t tot) : Tot (bitfields tot lo hi l) (decreases l) =
+inline_for_extraction
+noextract
+noeq
+type uint_t (tot: pos) (t: Type0) = {
+  v: (t -> Tot (U.uint_t tot));
+  uint_to_t: (U.uint_t tot -> Tot t);
+  v_uint_to_t: ((x: U.uint_t tot) -> Lemma (v (uint_to_t x) == x));
+  uint_to_t_v: ((x: t) -> Lemma (uint_to_t (v x) == x));
+  get_bitfield: ((x: t) -> (lo: nat) -> (hi: nat { lo <= hi /\ hi <= tot }) -> Tot (y: t { v y == BF.get_bitfield (v x) lo hi }));
+  set_bitfield: ((x: t) -> (lo: nat) -> (hi: nat { lo <= hi /\ hi <= tot }) -> (z: t { v z < pow2 (hi - lo) }) -> Tot (y : t { v y == BF.set_bitfield (v x) lo hi (v z)}));
+}
+
+let uint_t_v_uint_to_t #tot #t (cl: uint_t tot t) (x: U.uint_t tot) : Lemma
+  (cl.v (cl.uint_to_t x) == x)
+  [SMTPat (cl.v (cl.uint_to_t x))]
+= cl.v_uint_to_t x
+
+let uint_t_uint_to_t_v #tot #t (cl: uint_t tot t) (x: t) : Lemma
+  (cl.uint_to_t (cl.v x) == x)
+  [SMTPat (cl.uint_to_t (cl.v x))]
+= cl.uint_to_t_v x
+
+inline_for_extraction
+let bitfield (#tot: pos) (#t: Type0) (cl: uint_t tot t) (sz: nat { sz <= tot }) : Tot Type0 =
+  (x: t { cl.v x < pow2 sz })
+
+noextract
+let rec bitfields (#tot: pos) (#t: Type0) (cl: uint_t tot t) (lo: nat) (hi: nat { lo <= hi /\ hi <= tot }) (l: list nat { valid_bitfield_widths lo hi l }) : Tot Type0 (decreases l) =
+  match l with
+  | [] -> unit
+  | [sz] -> bitfield cl sz
+  | sz :: q -> bitfield cl sz & bitfields cl (lo + sz) hi q
+
+let rec synth_bitfield' (#tot: pos) (#t: Type0) (cl: uint_t tot t) (lo: nat) (hi: nat { lo <= hi /\ hi <= tot }) (l: list nat { valid_bitfield_widths lo hi l }) (x: t) : Tot (bitfields cl lo hi l) (decreases l) =
   match l with
   | [] -> ()
-  | [_] -> BF.get_bitfield x lo hi
-  | sz :: q -> (BF.get_bitfield x lo (lo + sz), synth_bitfield tot (lo + sz) hi q x)
+  | [_] -> cl.get_bitfield x lo hi
+  | sz :: q -> (((cl.get_bitfield x lo (lo + sz) <: t) <: bitfield cl sz), synth_bitfield' cl (lo + sz) hi q x)
 
-let rec synth_bitfield_injective (tot: pos) (lo: nat) (hi: nat { lo <= hi /\ hi <= tot }) (l: list nat { valid_bitfield_widths lo hi l }) (x y: U.uint_t tot) : Lemma
-  (requires (synth_bitfield tot lo hi l x == synth_bitfield tot lo hi l y))
-  (ensures (BF.get_bitfield x lo hi == BF.get_bitfield y lo hi))
+let synth_bitfield (#tot: pos) (#t: Type0) (cl: uint_t tot t) (lo: nat) (hi: nat { lo <= hi /\ hi <= tot }) (l: list nat { valid_bitfield_widths lo hi l }) (x: t) : Tot (bitfields cl lo hi l) = synth_bitfield' cl lo hi l x
+
+let rec synth_bitfield_injective' (#tot: pos) (#t: Type0) (cl: uint_t tot t) (lo: nat) (hi: nat { lo <= hi /\ hi <= tot }) (l: list nat { valid_bitfield_widths lo hi l }) (x y: t) : Lemma
+  (requires (synth_bitfield cl lo hi l x == synth_bitfield cl lo hi l y))
+  (ensures (BF.get_bitfield (cl.v x) lo hi == BF.get_bitfield (cl.v y) lo hi))
   (decreases l)
 = match l with
   | [] ->
-    BF.get_bitfield_empty x lo;
-    BF.get_bitfield_empty y lo
+    BF.get_bitfield_empty (cl.v x) lo;
+    BF.get_bitfield_empty (cl.v y) lo
   | [_] -> ()
   | sz :: q ->
-    synth_bitfield_injective tot (lo + sz) hi q x y;
-    BF.get_bitfield_partition_2_gen lo (lo + sz) hi x y
+    synth_bitfield_injective' cl (lo + sz) hi q x y;
+    BF.get_bitfield_partition_2_gen lo (lo + sz) hi (cl.v x) (cl.v y)
+
+let synth_bitfield_injective (#tot: pos) (#t: Type0) (cl: uint_t tot t) (lo: nat) (hi: nat { lo <= hi /\ hi <= tot }) (l: list nat { valid_bitfield_widths 0 tot l })
+  : Lemma ((lo == 0 /\ hi == tot) ==> synth_injective (synth_bitfield cl lo hi l))
+    [SMTPat (synth_injective (synth_bitfield #tot #t cl lo hi l))]
+=
+  synth_injective_intro' (synth_bitfield cl 0 tot l) (fun x y ->
+    synth_bitfield_injective' cl 0 tot l x y;
+    BF.get_bitfield_full (cl.v x);
+    BF.get_bitfield_full (cl.v y);
+    assert (cl.uint_to_t (cl.v x) == cl.uint_to_t (cl.v y)))
 
 #push-options "--z3rlimit 64"
 
-let rec synth_bitfield_ext (tot: pos) (lo: nat) (hi: nat { lo <= hi /\ hi <= tot }) (l: list nat { valid_bitfield_widths lo hi l }) (x y: U.uint_t tot) : Lemma
-  (requires (BF.get_bitfield x lo hi == BF.get_bitfield y lo hi))
-  (ensures (synth_bitfield tot lo hi l x == synth_bitfield tot lo hi l y))
+let rec synth_bitfield_ext (#tot: pos) (#t: Type0) (cl: uint_t tot t) (lo: nat) (hi: nat { lo <= hi /\ hi <= tot }) (l: list nat { valid_bitfield_widths lo hi l }) (x y: t) : Lemma
+  (requires (BF.get_bitfield (cl.v x) lo hi == BF.get_bitfield (cl.v y) lo hi))
+  (ensures (synth_bitfield cl lo hi l x == synth_bitfield cl lo hi l y))
   (decreases l)
 = match l with
-  | [] -> ()
-  | [_] -> ()    
+  | [] -> assert (synth_bitfield cl lo hi l x == synth_bitfield cl lo hi l y)
+  | [_] ->
+    assert (cl.uint_to_t (cl.v (cl.get_bitfield x lo hi)) == cl.uint_to_t (cl.v (cl.get_bitfield y lo hi)));
+    assert (synth_bitfield cl lo hi l x == synth_bitfield cl lo hi l y)
   | sz :: q ->
-    BF.get_bitfield_get_bitfield x lo hi 0 sz;
-    BF.get_bitfield_get_bitfield x lo hi sz (hi - lo);
-    BF.get_bitfield_get_bitfield y lo hi 0 sz;
-    BF.get_bitfield_get_bitfield y lo hi sz (hi - lo);
-    synth_bitfield_ext tot (lo + sz) hi q x y
+    BF.get_bitfield_get_bitfield (cl.v x) lo hi 0 sz;
+    BF.get_bitfield_get_bitfield (cl.v x) lo hi sz (hi - lo);
+    BF.get_bitfield_get_bitfield (cl.v y) lo hi 0 sz;
+    BF.get_bitfield_get_bitfield (cl.v y) lo hi sz (hi - lo);
+    assert (cl.uint_to_t (cl.v (cl.get_bitfield x lo (lo + sz))) == cl.uint_to_t (cl.v (cl.get_bitfield y lo (lo + sz))));
+    synth_bitfield_ext cl (lo + sz) hi q x y;
+    assert (synth_bitfield cl lo hi l x == synth_bitfield cl lo hi l y)
 
 #pop-options
 
-module U32 = FStar.UInt32
+let parse_bitfield (#t: Type0) (#k: parser_kind) (p: parser k t) (#tot: pos) (cl: uint_t tot t) (l: list nat { valid_bitfield_widths 0 tot l }) : Tot (parser k (bitfields cl 0 tot l)) =
+  p `parse_synth` synth_bitfield cl 0 tot l
 
-let synth_bitfield32 (l: list nat { valid_bitfield_widths 0 32 l }) (x: U32.t) : Tot (bitfields 32 0 32 l) =
-  synth_bitfield 32 0 32 l (U32.v x)
-
-let synth_bitfield32_injective (l: list nat { valid_bitfield_widths 0 32 l }) : Lemma
-  (synth_injective (synth_bitfield32 l))
-  [SMTPat (synth_injective (synth_bitfield32 l))]
-= synth_injective_intro' (synth_bitfield32 l) (fun x y ->
-    synth_bitfield_injective 32 0 32 l (U32.v x) (U32.v y);
-    BF.get_bitfield_full (U32.v x);
-    BF.get_bitfield_full (U32.v y)
-  )
-
-let parse_bitfield32 (l: list nat { valid_bitfield_widths 0 32 l }) : Tot (parser parse_u32_kind (bitfields 32 0 32 l)) =
-  parse_u32 `parse_synth` synth_bitfield32 l
-
-let rec synth_bitfield_recip (tot: pos) (lo: nat) (hi: nat { lo <= hi /\ hi <= tot }) (l: list nat { valid_bitfield_widths lo hi l }) (x: bitfields tot lo hi l) : Tot (U.uint_t tot) (decreases l) =
+let rec synth_bitfield_recip (#tot: pos) (#t: Type0) (cl: uint_t tot t) (lo: nat) (hi: nat { lo <= hi /\ hi <= tot }) (l: list nat { valid_bitfield_widths lo hi l }) (x: bitfields cl lo hi l) : Tot t (decreases l) =
   match l with
-  | [] -> 0
-  | [_] -> BF.set_bitfield 0 lo hi x
+  | [] -> cl.uint_to_t 0
+  | [_] -> cl.set_bitfield (cl.uint_to_t 0) lo hi x
   | sz :: q ->
-    let (hd, tl) = x <: (BF.bitfield tot sz & bitfields tot (lo + sz) hi q) in
-    BF.set_bitfield (synth_bitfield_recip tot (lo + sz) hi q tl) lo (lo + sz) hd
+    let (hd, tl) = x <: (bitfield cl sz & bitfields cl (lo + sz) hi q) in
+    cl.set_bitfield (synth_bitfield_recip cl (lo + sz) hi q tl) lo (lo + sz) hd
 
-#push-options "--z3rlimit 16"
+#push-options "--z3rlimit 64"
 
-let rec synth_bitfield_recip_inverse
-  (tot: pos) (lo: nat) (hi: nat { lo <= hi /\ hi <= tot }) (l: list nat { valid_bitfield_widths lo hi l }) (x: bitfields tot lo hi l)
+let rec synth_bitfield_recip_inverse'
+  (#tot: pos) (#t: Type0) (cl: uint_t tot t)
+  (lo: nat) (hi: nat { lo <= hi /\ hi <= tot }) (l: list nat { valid_bitfield_widths lo hi l }) (x: bitfields cl lo hi l)
 : Lemma
-  (ensures (synth_bitfield tot lo hi l (synth_bitfield_recip tot lo hi l x) == x))
+  (ensures (synth_bitfield cl lo hi l (synth_bitfield_recip cl lo hi l x) == x))
   (decreases l)
 = match l with
-  | [] -> ()
+  | [] ->
+    assert (synth_bitfield cl lo hi l (synth_bitfield_recip cl lo hi l x) == x)
   | [sz] ->
-    let x = x <: BF.bitfield tot sz in
-    BF.get_bitfield_set_bitfield_same 0 lo hi x
+    let x = x <: bitfield cl sz in
+    BF.get_bitfield_set_bitfield_same 0 lo hi (cl.v x);
+    assert (synth_bitfield cl lo hi l (synth_bitfield_recip cl lo hi l x) ==
+      cl.get_bitfield (cl.set_bitfield (cl.uint_to_t 0) lo hi x) lo hi);
+    assert (cl.uint_to_t (cl.v (cl.get_bitfield (cl.set_bitfield (cl.uint_to_t 0) lo hi x) lo hi)) == cl.uint_to_t (cl.v x));
+    assert (synth_bitfield cl lo hi l (synth_bitfield_recip cl lo hi l x) == x)
   | sz :: q ->
-    let (hd, tl) = x <: (BF.bitfield tot sz & bitfields tot (lo + sz) hi q) in
-    let y = synth_bitfield_recip tot (lo + sz) hi q tl in
-    BF.get_bitfield_set_bitfield_same y lo (lo + sz) hd;
-    BF.get_bitfield_set_bitfield_other y lo (lo + sz) hd (lo + sz) hi;
-    synth_bitfield_ext tot (lo + sz) hi q y (BF.set_bitfield y lo (lo + sz) hd);
-    synth_bitfield_recip_inverse tot (lo + sz) hi q tl
+    let (hd, tl) = x <: (bitfield cl sz & bitfields cl (lo + sz) hi q) in
+    let y = synth_bitfield_recip cl (lo + sz) hi q tl in
+    BF.get_bitfield_set_bitfield_same (cl.v y) lo (lo + sz) (cl.v hd);
+    BF.get_bitfield_set_bitfield_other (cl.v y) lo (lo + sz) (cl.v hd) (lo + sz) hi;
+    synth_bitfield_ext cl (lo + sz) hi q y (cl.set_bitfield y lo (lo + sz) hd);
+    synth_bitfield_recip_inverse' cl (lo + sz) hi q tl;
+    assert (cl.uint_to_t (cl.v (fst (synth_bitfield cl lo hi l (synth_bitfield_recip cl lo hi l x) <: (bitfield cl sz & bitfields cl (lo + sz) hi q)))) == cl.uint_to_t (cl.v (cl.get_bitfield (cl.set_bitfield (synth_bitfield_recip cl (lo + sz) hi q tl) lo (lo + sz) hd) lo (lo + sz))));
+    assert (synth_bitfield cl lo hi l (synth_bitfield_recip cl lo hi l x) == x)
 
 #pop-options
 
+(*
 let synth_bitfield32_recip
   (l: list nat { valid_bitfield_widths 0 32 l })
   (x: bitfields 32 0 32 l)
@@ -139,3 +177,69 @@ let serialize_bitfield32
     serialize_u32
     (synth_bitfield32_recip l)
     ()
+
+(*
+module U32 = FStar.UInt32
+module U64 = FStar.UInt64
+
+inline_for_extraction
+noextract
+let uint64 : uint_t 64 U64.t = {
+  v = U64.v;
+  uint_to_t = U64.uint_to_t;
+  v_uint_to_t = (fun _ -> ());
+  uint_to_t_v = (fun _ -> ());
+  get_bitfield = (fun x lo hi -> BF.get_bitfield64 x lo hi);
+  set_bitfield = (fun x lo hi z -> BF.set_bitfield64 x lo hi z);
+}
+
+inline_for_extraction
+noextract
+let uint32 : uint_t 32 U32.t = {
+  v = U32.v;
+  uint_to_t = U32.uint_to_t;
+  v_uint_to_t = (fun _ -> ());
+  uint_to_t_v = (fun _ -> ());
+  get_bitfield = (fun x lo hi -> BF.get_bitfield32 x lo hi);
+  set_bitfield = (fun x lo hi z -> BF.set_bitfield32 x lo hi z);
+}
+
+module U16 = FStar.UInt16
+module U8 = FStar.UInt8
+
+inline_for_extraction
+noextract
+let uint16 : uint_t 16 U16.t = {
+  v = U16.v;
+  uint_to_t = U16.uint_to_t;
+  v_uint_to_t = (fun _ -> ());
+  uint_to_t_v = (fun _ -> ());
+  get_bitfield = (fun x lo hi -> BF.get_bitfield16 x lo hi);
+  set_bitfield = (fun x lo hi z -> BF.set_bitfield16 x lo hi z);
+}
+
+inline_for_extraction
+noextract
+let uint8 : uint_t 8 U8.t = {
+  v = U8.v;
+  uint_to_t = U8.uint_to_t;
+  v_uint_to_t = (fun _ -> ());
+  uint_to_t_v = (fun _ -> ());
+  get_bitfield = (fun x lo hi -> BF.get_bitfield8 x lo hi);
+  set_bitfield = (fun x lo hi z -> BF.set_bitfield8 x lo hi z);
+}
+
+let synth_bitfield32 (l: list nat { valid_bitfield_widths 0 32 l }) (x: U32.t) : Tot (bitfields 32 0 32 l) =
+  synth_bitfield 32 0 32 l (U32.v x)
+
+let synth_bitfield32_injective (l: list nat { valid_bitfield_widths 0 32 l }) : Lemma
+  (synth_injective (synth_bitfield32 l))
+  [SMTPat (synth_injective (synth_bitfield32 l))]
+= synth_injective_intro' (synth_bitfield32 l) (fun x y ->
+    synth_bitfield_injective 32 0 32 l (U32.v x) (U32.v y);
+    BF.get_bitfield_full (U32.v x);
+    BF.get_bitfield_full (U32.v y)
+  )
+
+let parse_bitfield32 (l: list nat { valid_bitfield_widths 0 32 l }) : Tot (parser parse_u32_kind (bitfields 32 0 32 l)) =
+  parse_u32 `parse_synth` synth_bitfield32 l
